# Lecture 5

A = [
    3, 2, 2
    2, 3, 2
    2, 2, 3
]

A = [
    3-λ, 2, 2
    2, 3-λ, 2
    2, 2, 3-λ
]

-(λ - 1)²(λ - 7) = 0

λ = 1, λ = 7

* When λ = 1
  [
     2 2 2
     2 2 2
     2 2 2
  ] [
     x1
     x2
     x3
  ] = [
     2x1 + 2x2 + 2x3
     2x1 + 2x2 + 2x3
     2x1 + 2x2 + 2x3
  ] = 0

  = [
    1   1   1
    0   0   0
    0   0   0
  ]

  x + y + z = 0

* When λ = 7
  [
     -4 2 2
     2 -4 2
     2 2 -4
  ] [
     x1
     x2
     x3
  ] = [
     -4x1 + 2x2 + 2x3
     2x1 - 4x2 + 2x3
     2x1 + 2x2 - 4x3
  ] = 0

  = [
    1   1/2     1/2
    0   -6      6
    0   6       -6
  ]

    <!-- x + 1/2y + 1/2z = 0 -->
